rocq-skylabs-brick/theories/lang/cpp/syntax/mtraverse.v
@@ -230,6 +230,7 @@ Module MTraverse.
       | Estring s t => Estring s <$> ET (traverseT t)
       | Eint z t => Eint z <$> ET (traverseT t)
       | Ebool b => mret $ Ebool b
+      | Efloat ft v => mret $ Efloat ft v
       | Eunop o e t => Eunop o <$> traverseE e <*> ET (traverseT t)
       | Ebinop o e1 e2 t => Ebinop o <$> traverseE e1 <*> traverseE e2 <*> ET (traverseT t)
       | Ederef e t => Ederef <$> traverseE e <*> ET (traverseT t)
